---
id: vxVtPPyqf7rswiD9jeMrP
title: Rules of Differentiation
desc: ''
updated: 1643830380072
created: 1643828194844
---

- Notation
	- Prime notation
		- $f^′ (x)$
		- $y^\prime$
		- $f^′ $ 
		- Most common
	- Leibniz notation
		- $\frac{dy}{dx}$
		- $\frac{d}{dx} [y]$
	- Dot notation
		- $\dot{y}(t)$
		- $y\prime(t)$
	- Differentials
		- $D_x (f(x))$
- Constant rule
	- Let $f(x)=c$ where $c$ is a real number, then $\frac{dy}{dx} [c]=0$
- Identity derivative
	- Let $f(x)=x$, then $\frac{dy}{dx} [x]=1$
	- (If $f(x)$ equals itself, than the derivative of $x$ is $1$)
- Power rule
	- Let $f(x)=x^n$, where n is an unsigned (positive) integer, $\frac{dy}{dx} [x^n ]=nx^{n−1}$
- Constant multiple rule
	- Let $f(x)$ be a function and $c$ a constant, then $\frac{dy}{dx} [c∗f(x)]=c∗f′(x)$
- Sum and difference rule
	- Let $f(x)$ and $g(x)$ be functions, then $\frac{dy}{dx} [f(x)±g(x)]=f^′ (x)±g^′ (x)$
- Product Rule
	- $\frac{dy}{dx} [f(x)∗g(x)]=f^′ (x)g(x)+f(x)g′(x)$
- Quotient Rule
	- $\frac{dy}{dx} [\frac{f(x)}{g(x)} ]=\frac{f^′ (x)g(x)−f(x)g′(x)}{g(x)^2}$
- Sin Rule
	- $\frac{dy}{dx} [\sin{u}]=\cos{u}∗u′$
- Cosine Rule
	- $\frac{dy}{dx} [\cos{u} ]=−\sin({u})∗u^′$
- Tangent Rule
	- $\frac{dy}{dx} [\tan(u) ]=\sec^2(u)$
- Secant Rule
	- $\frac{dy}{dx} [\sec(x) ]=\sec(x)\tan(x)$
- Cosecant Rule
	- $\frac{dy}{dx} [\sec(x) ]=−\sec(x)\sec(x)$
- Cotangent Rule
	- $\frac{dy}{dx} [\sec(x) ]=−\sec^2⁡(x)$
- Euler's Number Rule
	- $\frac{dy}{dx} [e^u ]=e^u∗u′$
- Exponent Rule
	- $\frac{dy}{dx} [f(x)^{g(x)}  ]=g(x)∗f(x)^{g(x)−1}∗f′(x)$
	- Works w/ radicals too
- Function Rule (or polynomials)
	- $\frac{dy}{dx} [f(g(x))]=f^′ (g(x))∗g^′ (x)$
- Log Rules
	- $\frac{dy}{dx} [\ln(x) ]=1/x, x>0$
	- $\frac{dy}{dx} [\ln(|x|) ]=1/x, x≠0$
	- $\frac{dy}{dx} [\ln(g(x)) ]=\frac{1}{g(x)} ∗g^′ (x)=\frac{g^′ (x)}{g(x)}$
	- $\frac{dy}{dx} [ln⁡(c∗x) ]=1/x$ 
    ($c$ is a constant)
	- $\frac{dy}{dx} [\ln(x^n ) ]=\frac{n}{x}$
- General Exponential/Log Rule
	- $\frac{dy}{dx} [b^x ]=b^x∗ln⁡(b)$
	- $\frac{dy}{dx}[\log_b⁡(x)]=1/(\ln(b))$
- Inverse Sine Rule
	- $\frac{dy}{dx} [sin^{−1}(x) ]=1/\sqrt{1−x^2 }∗x′, −1<x<1$
- Inverse Cosine Rule
	- $\frac{dy}{dx} [\cos^{−1}(x)]=\frac{1}{\sqrt{1−x^2}}∗x′, −1<x<1$
- Inverse Tangent Rule
	- $\frac{dy}{dx} [\tan^{-1}(x)]=\frac{1}{1+x^2}∗x′$
- Inverse Secant Rule
	- $\frac{d}{dx}[sec^{-1}(x)]=\begin{cases}
        \frac{1}/{x\sqrt{x^2-1}}*x\prime &\text{, } x>1 \\
        -\frac{1}{x\sqrt{x^2-1}}*x\prime &\text{, } x<-1
    \end{cases}$
	- $\frac{dy}{dx} [sec^{-1}(x) ]=\frac{1}{|x| √(x^2−1)}, |x| > 1$
- Inverse Cosecant Rule
	- $\frac{dy}{dx} [\sec^{-1}(x) ]=−\frac{1}{|x| √(x^2−1)}∗x′$
- Inverse Cotangent Rule
	- $\frac{dy}{dx} [\sec^{−1}(x) ]=-\frac{1}{1+x^2}∗x′$
- General Inverse Trig Derivative
	- $\frac{dy}{dx} [trig^{−1} (g(x))]=\frac{1}{\sqrt{1−(g(x))^2}}∗g′(x)$
- General Inverse Function Derivative
	- $\frac{dy}{dx} [f^{-1} (x)]=\frac{1}{f′(f^{-1} (x))}$
	- $(f(x)=y \land f^{-1} (y)=x) \rarr \frac{dy}{dx} [f^{-1} (y)]=1/(f′(x))$

